{
 "cells": [
  {
   "cell_type": "markdown",
   "id": "ebfd2a09",
   "metadata": {},
   "source": [
    "# Proof of bisection method error bound\n",
    "## Kincaid & Cheney Section 3.1 Theorem 1\n",
    "\n",
    "**Theorem** If $(a_n)$ is the sequence of left endpoints, $(b_n)$ the sequence of right endpoints, and $(c_n)$ the sequence of midpoints in the bisection method, and if $a_n\\leq r\\leq b_n$ for all $n$, then\n",
    "$$|r - c_n|\\leq 2^{-(n+1)}|b_0 - a_0|$$\n",
    "\n",
    "*Proof.*  First, we make an important observation.  For all $n$,\n",
    "\n",
    "\\begin{align*}\n",
    "r - c_n &= r - \\frac{a_n + b_n}{2} \\\\\n",
    "\\end{align*}\n",
    "\n",
    "Since $r\\geq a_n$ for all $n$, we have\n",
    "\n",
    "\\begin{align*}\n",
    "r - c_n &\\geq a_n - \\frac{a_n + b_n}{2}\\\\\n",
    "&= \\frac{2a_n - a_n - b_n}{2}\\\\\n",
    "&= - \\frac{b_n - a_n}{2}\n",
    "\\end{align*}\n",
    "\n",
    "Since $r\\leq b_n$ for all $n$, we have\n",
    "\\begin{align*}\n",
    "r - c_n &\\leq b_n - \\frac{a_n + b_n}{2}\\\\\n",
    "&= \\frac{2b_n - a_n - b_n}{2}\\\\\n",
    "&= \\frac{b_n - a_n}{2}\n",
    "\\end{align*}\n",
    "\n",
    "Consequently,\n",
    "$$-\\frac{b_n - a_n}{2} \\leq r - c_n \\leq \\frac{b_n - a_n}{2}$$\n",
    "\n",
    "Or equivalently,\n",
    "$$|r - c_n| \\leq \\frac{b_n - a_n}{2}$$\n",
    "\n",
    "So it is sufficient to prove the following result:\n",
    "\n",
    "$$\\frac{b_n - a_n}{2} = 2^{-(n + 1)}(b_0 - a_0)$$\n",
    "for all $n$.\n",
    "\n",
    "Now we proceed by induction on $n$.\n",
    "\n",
    "*Base case*.  When $n = 0$, we have\n",
    "$$\\frac{b_0 - a_0}{2} = -2^{-(0 + 1)}(b_0 - a_0)$$\n",
    "\n",
    "*Inductive hypothesis*.  Suppose for some $k\\geq 0$,\n",
    "$$\\frac{b_k - a_k}{2} = 2^{-(k + 1)}(b_0 - a_0)$$\n",
    "\n",
    "**Case 1.** Suppose $a_{k+1} = a_k$ and $b_{k+1} = c_k = \\frac{a_k + b_k}{2}$.\n",
    "\n",
    "Then\n",
    "\\begin{align*}\n",
    "\\frac{b_{k+1} - a_{k+1}}{2} &= \\frac{\\frac{a_k + b_k}{2} - a_k}{2} \\\\\n",
    "&= \\frac{a_k + b_k - 2a_k}{4} \\\\\n",
    "&= \\frac{1}{2}\\cdot\\frac{b_k - a_k}{2}\\\\\n",
    "&= \\frac{1}{2}\\cdot 2^{-(k+1)}(b_0 - a_0) \\\\\n",
    "&= 2^{-(k+2)}(b_0 - a_0) \\\\\n",
    "\\end{align*}\n",
    "\n",
    "**Case 2.** Suppose $a_{k+1} = c_k = \\frac{a_k + b_k}{2}$ and $b_{k+1} = b_k$.\n",
    "\n",
    "Then\n",
    "\\begin{align*}\n",
    "\\frac{b_{k+1} - a_{k+1}}{2} &= \\frac{\\frac{b_k - a_k}{2} + b_k}{2} \\\\\n",
    "&= \\frac{b_k - a_k + 2b_k}{4} \\\\\n",
    "&= \\frac{1}{2}\\cdot\\frac{b_k - a_k}{2}\\\\\n",
    "&= \\frac{1}{2}\\cdot 2^{-(k+1)}(b_0 - a_0) \\\\\n",
    "&= 2^{-(k+2)}(b_0 - a_0) \\\\\n",
    "\\end{align*}\n",
    "\n",
    "We have now proved by induction that \n",
    "$$\\frac{b_n - a_n}{2} = 2^{-(n + 1)}(b_0 - a_0)$$,\n",
    "\n",
    "and since we have proved that $|r - c_n|\\leq \\frac{b_n - a_n}{2}$, it follows that\n",
    "$$|r - c_n|\\leq 2^{-(n+1)}|b_0 - a_0|$$\n",
    "for all $n$."
   ]
  }
 ],
 "metadata": {
  "kernelspec": {
   "display_name": "M2",
   "language": "text/x-macaulay2",
   "name": "m2"
  },
  "language_info": {
   "codemirror_mode": "macaulay2",
   "file_extension": ".m2",
   "mimetype": "text/x-macaulay2",
   "name": "Macaulay2"
  }
 },
 "nbformat": 4,
 "nbformat_minor": 5
}
