{
 "cells": [
  {
   "cell_type": "markdown",
   "id": "25540738",
   "metadata": {},
   "source": [
    "# Homework 6\n",
    "## Hermite Interpolation (Kincaid & Cheney Section 6.3)\n",
    "\n"
   ]
  },
  {
   "cell_type": "markdown",
   "id": "c98c7161",
   "metadata": {},
   "source": [
    "### Polynomial proof\n",
    "\n",
    "*Prove that if $n$ is a nonnegative integer, $p$ is a polynomial with degree greater than $n$, and $p^{(j)}(x_0) = 0$ for some $x_0\\in\\mathbb R$ and all $j\\in\\{0,\\ldots,n\\}$, then $(x - x_0)^{n+1}$ divides $p(x)$.*\n",
    "\n",
    "Suppose $\\deg p = m$.  By Taylor's theorem, for any $x$, there exists some $\\xi$ between $x$ and $x_0$ such that\n",
    "\\begin{equation*}\n",
    "p(x) = \\sum_{j=0}^m\\frac{p^{(j)}(x_0)}{j!}(x - x_0)^j + p^{(m+1)}(\\xi)(x - x_0)^{m + 1}\n",
    "\\end{equation*}\n",
    "\n",
    "Since $\\deg p=m$, $p^{(m+1)}(x) = 0$ for all $x$, and in particular, $p^{(m+1)}(\\xi) = 0$.  Also, since the lower order derivatives of $p$ all vanish at $x_0$ by assumption, this simplifies to\n",
    "\\begin{align*}\n",
    "p(x) &= \\sum_{j=n+1}^m\\frac{p^{(j)}(x_0)}{j!}(x - x_0)^j \\\\\n",
    "&= (x - x_0)^{n+1}\\sum_{j = n+1}^m\\frac{p^{(j)}(x_0)}{j!}(x - x_0)^{j - (n + 1)}\n",
    "\\end{align*}\n",
    "\n",
    "Consequently, $(x - x_0)^{n+1}$ divides $p(x)$."
   ]
  },
  {
   "cell_type": "markdown",
   "id": "9a26de2f",
   "metadata": {},
   "source": [
    "### Section 6.3 Problem 1\n",
    "We use the given information to construct the divided difference table below:\n",
    "\n",
    "\\begin{equation*}\n",
    "\\begin{array}{rr|rrrr}\n",
    "0 & 2 & -9  & \\frac{-6-(-9)}{1 - 0} = 3 & \\frac{10 - 3}{1 - 0} = 7 & \\frac{17 - 7}{2 - 0} = 5\\\\\n",
    "0 & 2 &  \\frac{-4-2}{1-0} = -6 & \\frac{4-(-6)}{1 - 0} = 10 & \\frac{44 - 10}{2 - 0} = 17\\\\\n",
    "1 & -4 & 4 & \\frac{48 - 4}{2 - 1} = 44 &\\\\\n",
    "1 & -4 & \\frac{44-(-4)}{2-1} = 48\\\\\n",
    "2 & 44 &\n",
    "\\end{array}\n",
    "\\end{equation*}\n",
    "\n",
    "Therefore, our Hermite polynomial is\n",
    "$$p(x) = 2 - 9x + 3x^2 + 7x^2(x - 1) + 5x^2(x - 1)^2$$"
   ]
  },
  {
   "cell_type": "markdown",
   "id": "c1f1caac",
   "metadata": {},
   "source": [
    "### Problem 2\n",
    "We add one more row at the bottom of our divided difference table from the previous problem to compute the coefficient of the new term:\n",
    "\\begin{equation*}\n",
    "\\begin{array}{rr|rrrrr}\n",
    "0 & 2 & -9  & \\frac{-6-(-9)}{1 - 0} = 3 & \\frac{10 - 3}{1 - 0} = 7 & \\frac{17 - 7}{2 - 0} = 5 &= \\frac{-20.5 - 5}{3-0}=-8.5\\\\\n",
    "0 & 2 &  \\frac{-4-2}{1-0} = -6 & \\frac{4-(-6)}{1 - 0} = 10 & \\frac{44 - 10}{2 - 0} = 17 & \\frac{-44.5-17}{3-0} = -20.5\\\\\n",
    "1 & -4 & 4 & \\frac{48 - 4}{2 - 1} = 44 & \\frac{-45 - 44}{3 - 1} = -44.5\\\\\n",
    "1 & -4 & \\frac{44-(-4)}{2-1} = 48 & \\frac{-42 - 48}{3 - 1} = -45 \\\\\n",
    "2 & 44 & \\frac{2 - 44}{3 - 2} = -42\\\\\n",
    "3 & 2 &\n",
    "\\end{array}\n",
    "\\end{equation*}\n",
    "\n",
    "Now adding this last term to our answer from above, we get:\n",
    "$$p(x) = 2 - 9x + 3x^2 + 7x^2(x - 1) + 5x^2(x - 1)^2-8.5x^2(x-1)^2(x-2)$$"
   ]
  },
  {
   "cell_type": "markdown",
   "id": "9081df54",
   "metadata": {},
   "source": [
    "### Problem 4\n",
    "\n",
    "Suppose we have a cubic polynomial $p$, i.e., $p(x) = a_3x^3 + a_2x^2 + a_1x + a_0$.  Then\n",
    "\\begin{align*}\n",
    "p'(x) &= 3a_3x^2 + 2a_2x + a_1 \\\\\n",
    "p''(x) &= 6a_3x + 2a_2\n",
    "\\end{align*}\n",
    "\n",
    "Plugging in $x_0$ and $x_1$, we have a system of four linear equations:\n",
    "\\begin{align*}\n",
    "a_3x_0^3 + a_2x_0^2 + a_1x_0 + a_0 &= c_{00} \\\\\n",
    "a_3x_1^3 + a_2x_1^2 + a_1x_1 + a_0 &= c_{10} \\\\\n",
    "6a_3x_0 + 2a_2 &= c_{02} \\\\\n",
    "6a_3x_1 + 2a_2 &= c_{12} \\\\\n",
    "\\end{align*}\n",
    "\n",
    "Or equivalently, \n",
    "\\begin{equation*}\n",
    "\\begin{pmatrix}\n",
    "x_0^3 & x_0^2 & x_0 & 1 \\\\\n",
    "x_1^3 & x_1^2 & x_1 & 1 \\\\\n",
    "6x_0 & 2 & 0 & 0 \\\\\n",
    "6x_1 & 2 & 0 & 0\n",
    "\\end{pmatrix}\n",
    "\\begin{pmatrix} a_3 \\\\ a_2 \\\\ a_1 \\\\ a_0\\end{pmatrix}\n",
    "=\n",
    "\\begin{pmatrix} c_{00} \\\\ c_{10} \\\\ c_{02} \\\\ c_{12}\\end{pmatrix}\n",
    "\\end{equation*}\n",
    "\n",
    "We know from linear algebra that this will have a solution for arbitrary $c_{ij}$ if and only if the coefficient matrix is invertible.  So let's compute its determinant.  Let's use cofactor expansion, taking advantage of as many 0's as we can:\n",
    "\n",
    "\\begin{align*}\n",
    "\\begin{vmatrix}\n",
    "x_0^3 & x_0^2 & x_0 & 1 \\\\\n",
    "x_1^3 & x_1^2 & x_1 & 1 \\\\\n",
    "6x_0 & 2 & 0 & 0 \\\\\n",
    "6x_1 & 2 & 0 & 0\n",
    "\\end{vmatrix}\n",
    "&= -1\\cdot \n",
    "\\begin{vmatrix}\n",
    "x_1^3 & x_1^2 & x_1 \\\\\n",
    "6x_0 & 2 & 0 \\\\\n",
    "6x_1 & 2 & 0 \n",
    "\\end{vmatrix}\n",
    "+ 1\\cdot\n",
    "\\begin{vmatrix}\n",
    "x_0^3 & x_0^2 & x_0 \\\\\n",
    "6x_0 & 2 & 0 \\\\\n",
    "6x_1 & 2 & 0\n",
    "\\end{vmatrix} \\\\\n",
    "&= -x_1\\begin{vmatrix}\n",
    "6x_0 & 2 \\\\\n",
    "6x_1 & 2 \n",
    "\\end{vmatrix}\n",
    "+x_0\\begin{vmatrix}\n",
    "6x_0 & 2 \\\\\n",
    "6x_1 & 2 \n",
    "\\end{vmatrix} \\\\\n",
    "&= -x_1(12x_0 - 12x_1) + x_0(12x_0 - 12x_1) \\\\\n",
    "&= 12(x_0 - x_1)^2\n",
    "\\end{align*}\n",
    "\n",
    "This determinant only vanishes when $x_0=x_1$, and so we are guaranteed a cubic solution provided that our nodes are distinct.\n",
    "\n",
    "\n"
   ]
  },
  {
   "cell_type": "markdown",
   "id": "5a58d77b",
   "metadata": {},
   "source": [
    "### Problem 5\n",
    "\n",
    "Let's start with equation (6):\n",
    "\n",
    "\\begin{equation*}\n",
    "p(x) = p(x_0) + p[x_0,x_0](x - x_0) + p[x_0,x_0,x_1](x - x_0)^2\n",
    "\\end{equation*}\n",
    "\n",
    "Now substitute in the values from equation and (5) and recalling that $p(x_0=c_{00}$ and $p[x_0,x_0] = p'(x_0) = c_{01}$:\n",
    "\\begin{equation*}\n",
    "p(x) = c_{00} + c_{01}(x - x_0) + \\left(\\frac{c_{10}-c_{00}}{(x_1-x_0)^2} - \\frac{c_{01}}{x_1 - x_0}\\right)(x - x_0)^2\n",
    "\\end{equation*}\n",
    "\n",
    "When plugging in $x = x_0$, the last two terms vanish, leaving $p(x_0)=c_{00}$ as desired.  \n",
    "Also:\n",
    "\\begin{align*}\n",
    "p(x_1) &= c_{00} + c_{01}(x_1 - x_0) + \\left(\\frac{c_{10}-c_{00}}{(x_1-x_0)^2} - \\frac{c_{01}}{x_1 - x_0}\\right)(x_1 - x_0)^2 \\\\\n",
    "&= c_{00} + c_{01}(x_1 - x_0) + c_{10}-c_{00} - c_{01}(x_1 - x_0) \\\\\n",
    "&= c_{10}\n",
    "\\end{align*}\n",
    "\n",
    "Now, differentiating:\n",
    "\\begin{align*}\n",
    "p'(x) &= c_{01}+2\\left(\\frac{c_{10}-c_{00}}{(x_1-x_0)^2} - \\frac{c_{01}}{x_1 - x_0}\\right)(x - x_0) \\\\\n",
    "\\end{align*}\n",
    "\n",
    "When plugging in $x = x_0$, the second term vanishes, leaving $p'(x_0)=c_{01}$ as desired.\n",
    "\n"
   ]
  },
  {
   "cell_type": "markdown",
   "id": "230c2942",
   "metadata": {},
   "source": [
    "## Spline Interpolation (Section 6.4)\n",
    "### Problem 13\n",
    "First, let's check that the function interpolates the data:\n",
    "\\begin{align*}\n",
    "f(0) &= 1 + 0 - 0^3 = 1 \\\\\n",
    "f(1) &= 1 + 1 - 1^3 = 1 \\text{ (from the left)}\\\\\n",
    "f(1) &= 1 - 2(1 - 1) - 3(1 - 1)^2 + 4(1-1)^3 = 1\\text{ (from the right)} \\\\\n",
    "f(2) &= 1 - 2(2 - 1) - 3(2 - 1)^2 + 4(2-1)^3 = 0\\text{ (from the left)} \\\\\n",
    "f(2) &= 4(2 -2 ) + 9(2 - 2)^2 - 3(2 -2 )^3 = 0\\text{ (from the right)} \\\\\n",
    "f(3) &= 4(3 -2 ) + 9(3 - 2)^2 - 3(3 -2 )^3 = 10\n",
    "\\end{align*}\n",
    "\n",
    "So far so good.\n",
    "\n",
    "Now let's check that the derivatives agree:\n",
    "\\begin{align*}\n",
    "f'(x) &= \\begin{cases}\n",
    "1 - 3x^2 &\\text{ if 0 < $x$ < 1 } \\\\\n",
    "-2 -6(x - 1) + 12(x-1)^2 &\\text{ if 1 < $x$ < 2 } \\\\\n",
    "4 + 18(x - 2) -9(x - 2)^2&\\text{ if 2 < $x$ < 3 }\n",
    "\\end{cases}\n",
    "\\end{align*}\n",
    "\n",
    "At $x = 1$, the first two both evaluate to $-2$, and at $x=2$, the last two both evaluate to $4$.\n",
    "\n",
    "Finally, let's check the second derivatives:\n",
    "\\begin{align*}\n",
    "f''(x) &= \\begin{cases}\n",
    "-6x &\\text{ if 0 < $x$ < 1 } \\\\\n",
    "-6 + 24(x-1) &\\text{ if 1 < $x$ < 2 } \\\\\n",
    "18-18(x - 2)&\\text{ if 2 < $x$ < 3 }\n",
    "\\end{cases}\n",
    "\\end{align*}\n",
    "The first one vanishes at 0, and the first two both evaluate to $-6$ at 1.  The last two both evaluate to 18 at 2, and the last one vanishes at 3.\n",
    "\n",
    "**YES**.  This is a natural cubic spline for the given data.\n"
   ]
  },
  {
   "cell_type": "markdown",
   "id": "0f6a2e1e",
   "metadata": {},
   "source": [
    "### Problem 14\n",
    "Let's check that the component polynomials agree on each interior knot:\n",
    "\n",
    "\\begin{align*}\n",
    "f(0) &= 2(0+1) + (0+1)^3 = 3 \\text{ (from the left)} \\\\\n",
    "f(0) &= 3 + 5\\cdot 0 + 3\\cdot 0^2 = 3 \\text{ (from the right)} \\\\\n",
    "f(1) &= 3 + 5\\cdot 1 + 3\\cdot 1^2 = 11 \\text{ (from the left)} \\\\\n",
    "f(1) &= 11 + 11(11- 1) + 3(11 - 1)^2 - (11 - 1)^3 = 11\\text{ (from the right)}\n",
    "\\end{align*}\n",
    "\n",
    "Now let's check the derivatives:\n",
    "\\begin{equation*}\n",
    "f'(x) = \\begin{cases}\n",
    "2 + 3(x+1)^2 &\\text{if }-1<x<0 \\\\\n",
    "5 + 6x &\\text{if }0 < x < 1 \\\\\n",
    "11 + 6(x - 1) - 3(x-1)^2&\\text{if }1 < x < 2\n",
    "\\end{cases}\n",
    "\\end{equation*}\n",
    "\n",
    "So\n",
    "\\begin{align*}\n",
    "f'(0) &= 2 + 3(0+1)^2 = 5\\text{ (from the left)} \\\\\n",
    "f'(0) &= 5 + 6\\cdot 0 = 5\\text{ (from the right)} \\\\\n",
    "f'(1) &= 5 + 6\\cdot 1 = 11 \\text{ (from the left)} \\\\\n",
    "f'(1) &= 11 + 6(1 - 1) - 3(1-1)^2 = 11\\text{ (from the right)}\n",
    "\\end{align*}\n",
    "\n",
    "And finally, the second derivatives:\n",
    "\\begin{equation*}\n",
    "f''(x) = \\begin{cases}\n",
    "6(x+1)       &\\text{if }-1 < x < 0 \\\\\n",
    "6            &\\text{if } 0 < x < 1 \\\\\n",
    "6 - 6(x - 1) &\\text{if } 1 < x < 2\n",
    "\\end{cases}\n",
    "\\end{equation*}\n",
    "\n",
    "This gives us\n",
    "\\begin{align*}\n",
    "f''(-1) &= 6(-1+1) = 0 \\\\\n",
    "f''(0) &= 6(0+1) = 6\\text{ (from the left)} \\\\\n",
    "f''(0) &= 6\\text{ (from the right)} \\\\\n",
    "f''(1) &= 6\\text{ (from the left)} \\\\\n",
    "f''(1) &= 6 - 6(1 - 1) = 6\\text{ (from the right)} \\\\\n",
    "f''(2) &= 6 - 6(2 - 1) = 0\n",
    "\\end{align*}\n",
    "\n",
    "**YES**.  This is a natural cubic spline."
   ]
  },
  {
   "cell_type": "markdown",
   "id": "14102c88",
   "metadata": {},
   "source": [
    "### Problem 17\n",
    "Let's suppose that $S''(0) = z$.  Since we want $S''(-1) = S''(1) = 0$, we start with the following:\n",
    "\n",
    "\\begin{align*}\n",
    "S_0''(x) &= 0\\cdot\\frac{x - 0}{-1 - 0} + z\\cdot \\frac{x - (-1)}{0 - (-1)} \\\\\n",
    "&= z(x + 1) \\\\\n",
    "S_1''(x) &= z\\cdot\\frac{x - 1}{0 - 1} + 0\\cdot\\frac{x - 0)}{1 - 0} \\\\\n",
    "&= -z(x - 1)\n",
    "\\end{align*}\n",
    "\n",
    "Integrating twice, we get:\n",
    "\\begin{align*}\n",
    "S_0'(x) &= \\frac{z}{2}(x + 1)^2 + C_0\\\\\n",
    "S_0(x) &= \\frac{z}{6}(x + 1)^3 + C_0x + D_0\\\\\n",
    "S_1'(x) &= -\\frac{z}{2}(x - 1)^2 + C_1 \\\\\n",
    "S_1(x) &= -\\frac{z}{6}(x - 1)^3 + C_1x + D_1\n",
    "\\end{align*}\n",
    "\n",
    "Since we want $S_0(-1) = 13$, $S_0(0) = S_1(0) = 7$, $S_1(1) = 9$, and $S_0'(0) = S_1'(0)$, we have the following five equations:\n",
    "\n",
    "\\begin{align*}\n",
    "\\frac{z}{6}(-1 + 1)^3 + C_0(-1) + D_0 = 13 &\\implies -C_0 + D_0 = 13 \\\\\n",
    "\\frac{z}{6}(0 + 1)^3 + C_0\\cdot 0 + D_0 = 7 &\\implies \\frac{1}{6} z + D_0 = 7 \\\\\n",
    "-\\frac{z}{6}(0 - 1)^3 + C_1\\cdot 0 + D_1 = 7 &\\implies \\frac{1}{6} z + D_1 = 7 \\\\\n",
    "-\\frac{z}{6}(1 - 1)^3 + C_1\\cdot 1 + D_1 = 9 &\\implies C_1 + D_1 = 9 \\\\\n",
    "\\frac{z}{2}(0 + 1)^2 + C_0 = -\\frac{z}{2}(0 - 1)^2 + C_1 &\\implies z + C_0 - C_1 = 0\n",
    "\\end{align*}\n",
    "\n",
    "So we would like to solve the matrix equation\n",
    "\\begin{equation*}\n",
    "\\begin{pmatrix}\n",
    "0 & -1 & 1 & 0 & 0 \\\\\n",
    "\\frac{1}{6} & 0 & 1 & 0 & 0 \\\\\n",
    "\\frac{1}{6} & 0 & 0 & 0 & 1 \\\\\n",
    "0 & 0 & 0 & 1 & 1 \\\\\n",
    "1 & 1 & 0 & -1 & 0\n",
    "\\end{pmatrix}\n",
    "\\begin{pmatrix} z \\\\ C_0 \\\\ D_0 \\\\ C_1 \\\\ D_1\\end{pmatrix}\n",
    "= \\begin{pmatrix} 13 \\\\ 7 \\\\ 7 \\\\ 9 \\\\ 0\\end{pmatrix}\n",
    "\\end{equation*}\n",
    "\n",
    "Now let's solve this in Macaulay2:"
   ]
  },
  {
   "cell_type": "code",
   "execution_count": 8,
   "id": "372b9775",
   "metadata": {},
   "outputs": [
    {
     "name": "stdout",
     "output_type": "stream",
     "text": [
      "\n",
      "o8 = | 12 |\n",
      "     | -8 |\n",
      "     |  5 |\n",
      "     |  4 |\n",
      "     |  5 |\n",
      "\n",
      "       5\n",
      "o8 : QQ\n",
      "\u001b[?2004h"
     ]
    }
   ],
   "source": [
    "A = matrix {{0, -1, 1, 0, 0}, {1/6, 0, 1, 0, 0}, {1/6, 0, 0, 0, 1}, {0, 0, 0, 1, 1}, {1, 1, 0, -1, 0}}\n",
    "b = vector {13, 7, 7, 9, 0/1}\n",
    "solve(A, b)"
   ]
  },
  {
   "cell_type": "markdown",
   "id": "f68f8c02",
   "metadata": {},
   "source": [
    "So we have\n",
    "\\begin{align*}\n",
    "S_0(x) &= \\frac{12}{6}(x + 1)^3 -8x + 5 = 2(x + 1)^3 - 8x + 5\\\\\n",
    "S_1(x) &= -\\frac{12}{6}(x - 1)^3 + 4x + 5 = -2(x - 1)^3 + 4x + 5\n",
    "\\end{align*}"
   ]
  },
  {
   "cell_type": "markdown",
   "id": "fc438166",
   "metadata": {},
   "source": [
    "### Problem 18\n",
    "First, let's check that the two components agree at the knot 0:\n",
    "\n",
    "\\begin{align*}\n",
    "f(0) &= (0+1) + (0+1)^3 = 2\\text{ (from the left)} \\\\\n",
    "f(0) &= 4 + (0 -1 ) + (0 - 1)^3 = 2 \\text{ (from the right)} \\\\\n",
    "\\end{align*}\n",
    "\n",
    "Now let's check the derivatives:\n",
    "\\begin{equation*}\n",
    "f'(x) = \\begin{cases}\n",
    "1 + 3(x+1)^2 &\\text{if }-1 \\leq x < 0 \\\\\n",
    "1 + 3(x - 1)^2&\\text{if } 0 < x \\leq 1\n",
    "\\end{cases}\n",
    "\\end{equation*}\n",
    "On both the left and the right, $f'(x)\\to 4$ as $x\\to 0$.  So far so good.\n",
    "\n",
    "Finally, let's check the second derivatives:\n",
    "\\begin{equation*}\n",
    "f''(x) = \\begin{cases}\n",
    "6(x + 1) &\\text{if }-1 \\leq x < 0 \\\\\n",
    "6(x - 1) &\\text{if }0 < x \\leq 1\n",
    "\\end{cases}\n",
    "\\end{equation*}\n",
    "\n",
    "We have $f''(-1) = f''(1) = 0$, as desired.  However, $\\lim_{x\\to 0^-}f''(x)=6$ but $\\lim_{x\\to 0^+}f''(x) = -6$.  Since the second derivatives do not agree at 0, this is **NOT** a natural cubic spline.\n"
   ]
  },
  {
   "cell_type": "markdown",
   "id": "608e42ee",
   "metadata": {},
   "source": [
    "### Problem 19\n",
    "Note that this problem is nearly identical to Problem 17 since the knots agree.  We only need to change the value of the spline at the knot $-1$ from 13 to 5.  After doing the same setup as before and swapping in the new value, we end up with the following linear system:\n",
    "\\begin{equation*}\n",
    "\\begin{pmatrix}\n",
    "0 & -1 & 1 & 0 & 0 \\\\\n",
    "\\frac{1}{6} & 0 & 1 & 0 & 0 \\\\\n",
    "\\frac{1}{6} & 0 & 0 & 0 & 1 \\\\\n",
    "0 & 0 & 0 & 1 & 1 \\\\\n",
    "1 & 1 & 0 & -1 & 0\n",
    "\\end{pmatrix}\n",
    "\\begin{pmatrix} z \\\\ C_0 \\\\ D_0 \\\\ C_1 \\\\ D_1\\end{pmatrix}\n",
    "= \\begin{pmatrix} 5 \\\\ 7 \\\\ 7 \\\\ 9 \\\\ 0\\end{pmatrix}\n",
    "\\end{equation*}\n",
    "\n",
    "Solving this system in Macaulay2:\n"
   ]
  },
  {
   "cell_type": "code",
   "execution_count": 12,
   "id": "7901f053",
   "metadata": {},
   "outputs": [
    {
     "name": "stdout",
     "output_type": "stream",
     "text": [
      "\n",
      "o12 = | 0 |\n",
      "      | 2 |\n",
      "      | 7 |\n",
      "      | 2 |\n",
      "      | 7 |\n",
      "\n",
      "        5\n",
      "o12 : QQ\n",
      "\u001b[?2004h"
     ]
    }
   ],
   "source": [
    "A = matrix {{0, -1, 1, 0, 0}, {1/6, 0, 1, 0, 0}, {1/6, 0, 0, 0, 1}, {0, 0, 0, 1, 1}, {1, 1, 0, -1, 0}}\n",
    "b = vector(QQ^5, {5, 7, 7, 9, 0})\n",
    "solve(A, b)"
   ]
  },
  {
   "cell_type": "markdown",
   "id": "afce565d",
   "metadata": {},
   "source": [
    "Consequently, our natural cubic spline is:\n",
    "\\begin{align*}\n",
    "S_0(x) &= \\frac{0}{6}(x + 1)^3 + 2x + 7 = 2x + 7 \\\\\n",
    "S_1(x) &= -\\frac{0}{6}(x - 1)^3 + 2x + 7 = 2x + 7\n",
    "\\end{align*}\n",
    "\n",
    "And in fact, the function we are interpolating is just the linear function $f(x) = 2x + 7$."
   ]
  }
 ],
 "metadata": {
  "kernelspec": {
   "display_name": "M2",
   "language": "text/x-macaulay2",
   "name": "m2"
  },
  "language_info": {
   "codemirror_mode": "macaulay2",
   "file_extension": ".m2",
   "mimetype": "text/x-macaulay2",
   "name": "Macaulay2"
  }
 },
 "nbformat": 4,
 "nbformat_minor": 5
}
